src/Ex/Mesi/MesiInvInv1.v
@@ -19,6 +19,680 @@ Local Open Scope fmap.
 
 Existing Instance Mesi.ImplOStateIfc.
 
+Definition ObjDirMETo (ost: OState) (cidx: IdxT) :=
+  mesiE <= ost#[dir].(dir_st) <= mesiM /\
+  ost#[dir].(dir_excl) = cidx.
+
+Lemma getDir_I_ObjDirMETo_false:
+  forall oidx (ost: OState),
+    getDir oidx (fst (snd (snd (snd ost)))) = mesiI ->
+    ObjDirMETo ost oidx -> False.
+Proof.
+  unfold getDir, ObjDirMETo; intros; dest.
+  simpl in H.
+  do 2 (find_if_inside; [find_if_inside; [discriminate|auto]|]).
+  do 2 (find_if_inside; [simpl in *; solve_mesi|]).
+  discriminate.
+Qed.
+
+Definition InvDirME (topo: DTree) (st: MState): Prop :=
+  forall oidx pidx,
+    parentIdxOf topo oidx = Some pidx ->
+    _ <+- (bst_oss st)@[oidx]; (* need to know the existence of the child object *)
+      _ <+- (bst_orqs st)@[oidx];
+      post <+- (bst_oss st)@[pidx];
+      (ObjDirMETo post oidx -> NoRsI oidx (bst_msgs st)).
+
+Section InvDirME.
+  Variable (tr: tree).
+  Hypothesis (Htr: tr <> Node nil).
+
+  Let topo: DTree := fst (tree2Topo tr 0).
+  Let cifc: CIfc := snd (tree2Topo tr 0).
+  Let impl: System := impl Htr.
+
+  Lemma mesi_InvDirME_init:
+    Invariant.InvInit impl (InvDirME topo).
+  Proof.
+    do 2 (red; simpl); intros.
+    destruct (implOStatesInit tr)@[oidx] as [ost|] eqn:Host; simpl; auto.
+    destruct (implORqsInit tr)@[oidx] as [orq|] eqn:Horq; simpl; auto.
+    destruct (implOStatesInit tr)@[pidx] as [post|] eqn:Hpost; simpl; auto.
+    intros; exfalso.
+    red in H0; dest.
+    destruct (in_dec idx_dec pidx (c_li_indices cifc ++ c_l1_indices cifc)).
+    - subst cifc; rewrite c_li_indices_head_rootOf in i by assumption.
+      inv i.
+      + rewrite implOStatesInit_value_root in Hpost by assumption.
+        inv Hpost.
+        simpl in *; solve_mesi.
+      + rewrite implOStatesInit_value_non_root in Hpost by assumption.
+        inv Hpost.
+        simpl in *; solve_mesi.
+    - rewrite implOStatesInit_None in Hpost by assumption.
+      discriminate.
+  Qed.
+
+  Lemma mesi_InvDirME_ext_in:
+    forall oss orqs msgs,
+      InvDirME topo {| bst_oss := oss; bst_orqs := orqs; bst_msgs := msgs |} ->
+      InObjInds tr 0 {| bst_oss := oss; bst_orqs := orqs; bst_msgs := msgs |} ->
+      forall eins,
+        ValidMsgsExtIn impl eins ->
+        InvDirME topo {| bst_oss := oss; bst_orqs := orqs; bst_msgs := enqMsgs eins msgs |}.
+  Proof.
+    red; simpl; intros.
+    specialize (H _ _ H2); simpl in H.
+    destruct (oss@[oidx]) as [ost|] eqn:Host; simpl in *; auto.
+    destruct (orqs@[oidx]) as [orq|] eqn:Horq; simpl in *; auto.
+    destruct (oss@[pidx]) as [post|] eqn:Hpost; simpl in *; auto.
+    intros; specialize (H H3); dest.
+
+    apply MsgsP_other_midx_enqMsgs; [assumption|].
+    destruct H1; simpl.
+    eapply DisjList_SubList; [eassumption|].
+    eapply DisjList_comm, DisjList_SubList.
+    - eapply SubList_trans;
+        [|eapply tree2Topo_obj_chns_minds_SubList with (oidx:= oidx)].
+      + solve_SubList.
+      + specialize (H0 oidx); simpl in H0.
+        rewrite Host in H0; simpl in H0.
+        eassumption.
+    - apply tree2Topo_minds_merqs_disj.
+  Qed.
+
+  Lemma mesi_InvDirME_ext_out:
+    forall oss orqs msgs,
+      InvDirME topo {| bst_oss := oss; bst_orqs := orqs; bst_msgs := msgs |} ->
+      InObjInds tr 0 {| bst_oss := oss; bst_orqs := orqs; bst_msgs := msgs |} ->
+      forall (eouts: list (Id Msg)),
+        InvDirME topo {| bst_oss := oss;
+                         bst_orqs := orqs;
+                         bst_msgs := deqMsgs (idsOf eouts) msgs |}.
+  Proof.
+    red; simpl; intros.
+    specialize (H _ _ H1); simpl in H.
+    destruct (oss@[oidx]) as [ost|] eqn:Host; simpl in *; auto.
+    destruct (orqs@[oidx]) as [orq|] eqn:Horq; simpl in *; auto.
+    destruct (oss@[pidx]) as [post|] eqn:Hpost; simpl in *; auto.
+    intros; specialize (H H2); dest.
+    apply MsgsP_deqMsgs; assumption.
+  Qed.
+
+  Lemma InvDirME_other_msg_id_enqMP:
+    forall oss orqs msgs,
+      InvDirME topo {| bst_oss:= oss; bst_orqs:= orqs; bst_msgs:= msgs |} ->
+      forall midx msg,
+        msg.(msg_id) <> mesiInvRs ->
+        InvDirME topo {| bst_oss:= oss; bst_orqs:= orqs;
+                         bst_msgs:= enqMP midx msg msgs |}.
+  Proof.
+    red; simpl; intros.
+    specialize (H _ _ H1); simpl in H.
+    destruct (oss@[oidx]) as [ost|] eqn:Host; simpl in *; auto.
+    destruct (orqs@[oidx]) as [orq|] eqn:Horq; simpl in *; auto.
+    destruct (oss@[pidx]) as [post|] eqn:Hpost; simpl in *; auto.
+    intros.
+    apply MsgsP_other_msg_id_enqMP.
+    - apply H; auto.
+    - simpl; intro Hx.
+      destruct Hx; auto.
+  Qed.
+  
+  Lemma InvDirME_other_msg_id_enqMsgs:
+    forall oss orqs msgs,
+      InvDirME topo {| bst_oss:= oss; bst_orqs:= orqs; bst_msgs:= msgs |} ->
+      forall nmsgs,
+        Forall (fun idm => (valOf idm).(msg_id) <> mesiInvRs /\
+                           (valOf idm).(msg_id) <> mesiRsS) nmsgs ->
+        InvDirME topo {| bst_oss:= oss; bst_orqs:= orqs;
+                         bst_msgs:= enqMsgs nmsgs msgs |}.
+  Proof.
+    intros.
+    generalize dependent msgs.
+    induction nmsgs as [|[nmidx nmsg] nmsgs]; simpl; intros; auto.
+    inv H0; dest.
+    apply IHnmsgs; auto.
+    apply InvDirME_other_msg_id_enqMP; assumption.
+  Qed.
+
+  Lemma InvDirME_deqMP:
+    forall oss orqs msgs,
+      InvDirME topo {| bst_oss:= oss; bst_orqs:= orqs; bst_msgs:= msgs |} ->
+      forall midx,
+        InvDirME topo {| bst_oss:= oss; bst_orqs:= orqs;
+                         bst_msgs:= deqMP midx msgs |}.
+  Proof.
+    unfold InvDirME; simpl; intros.
+    specialize (H _ _ H0).
+    destruct (oss@[oidx]) as [ost|] eqn:Host; simpl in *; auto.
+    destruct (orqs@[oidx]) as [orq|] eqn:Horq; simpl in *; auto.
+    destruct (oss@[pidx]) as [post|] eqn:Hpost; simpl in *; auto.
+    intros; specialize (H H1); dest.
+    apply MsgsP_deqMP; assumption.
+  Qed.
+
+  Lemma InvDirME_deqMsgs:
+    forall oss orqs msgs,
+      InvDirME topo {| bst_oss:= oss; bst_orqs:= orqs; bst_msgs:= msgs |} ->
+      forall minds,
+        InvDirME topo {| bst_oss:= oss; bst_orqs:= orqs;
+                      bst_msgs:= deqMsgs minds msgs |}.
+  Proof.
+    unfold InvDirME; simpl; intros.
+    specialize (H _ _ H0).
+    destruct (oss@[oidx]) as [ost|] eqn:Host; simpl in *; auto.
+    destruct (orqs@[oidx]) as [orq|] eqn:Horq; simpl in *; auto.
+    destruct (oss@[pidx]) as [post|] eqn:Hpost; simpl in *; auto.
+    intros; specialize (H H1); dest.
+    apply MsgsP_deqMsgs; assumption.
+  Qed.
+
+  Ltac simpl_InvDirME_msgs_enqMP :=
+    simpl;
+    try match goal with
+        | [H: msg_id ?rmsg = _ |- msg_id ?rmsg <> _] => rewrite H
+        end;
+    discriminate.
+
+  Ltac simpl_InvDirME_msgs_enqMsgs :=
+    let idm := fresh "idm" in
+    let Hin := fresh "H" in
+    apply Forall_forall; intros idm Hin;
+    apply in_map_iff in Hin; dest; subst;
+    split; simpl_InvDirME_msgs_enqMP.
+
+  Ltac simpl_InvDirME_msgs :=
+    repeat
+      (first [apply InvDirME_other_msg_id_enqMP; [|simpl_InvDirME_msgs_enqMP..]
+             |apply InvDirME_other_msg_id_enqMsgs; [|simpl_InvDirME_msgs_enqMsgs]
+             |apply InvDirME_deqMP
+             |apply InvDirME_deqMsgs
+             |assumption]).
+
+  Ltac disc_bind_true :=
+    repeat
+      match goal with
+      | |- _ <+- ?ov; _ =>
+        first [match goal with
+               | [H: ov = _ |- _] => rewrite H in *; simpl in *
+               end
+              |let Hov := fresh "H" in
+               let v := fresh "v" in
+               destruct ov as [v|] eqn:Hov; simpl in *; [|auto]]
+      end.
+
+  Ltac disc_InvDirME :=
+    repeat
+      match goal with
+      | [Hi: InvDirME _ _ |- InvDirME _ _] =>
+        let Hp := fresh "H" in
+        red; simpl; intros ? ? Hp;
+        specialize (Hi _ _ Hp); simpl in Hi;
+        mred; simpl;
+        try (exfalso; eapply parentIdxOf_not_eq; subst topo; eauto; fail)
+      | |- _ <+- _; _ => disc_bind_true
+      end.
+
+  Lemma mesi_InvDirME_step:
+    Invariant.InvStep impl step_m (InvDirME topo).
+  Proof. (* SKIP_PROOF_OFF *)
+    red; intros.
+    pose proof (footprints_ok
+                  (mesi_GoodORqsInit Htr)
+                  (mesi_GoodRqRsSys Htr) H) as Hftinv.
+    pose proof (mesi_InObjInds H) as Hioi.
+    pose proof (mesi_MsgConflictsInv
+                  (@mesi_RootChnInv_ok _ Htr) H) as Hpmcf.
+    (* pose proof (mesi_MsgConflictsInv *)
+    (*               (@mesi_RootChnInv_ok _ Htr) *)
+    (*               (reachable_steps H (steps_singleton H1))) as Hnmcf. *)
+    pose proof (MesiDownLockInv_ok H) as Hmdl.
+    (* pose proof (mesi_InvWBDir_ok H) as Hidir. *)
+    inv H1; [assumption
+            |apply mesi_InvDirME_ext_in; auto
+            |apply mesi_InvDirME_ext_out; auto
+            |].
+
+    simpl in H2; destruct H2; [subst|apply in_app_or in H1; destruct H1].
+    
+    - (*! Cases for the main memory *)
+
+      (** Abstract the root. *)
+      assert (In (rootOf (fst (tree2Topo tr 0)))
+                 (c_li_indices (snd (tree2Topo tr 0)))) as Hin.
+      { rewrite c_li_indices_head_rootOf by assumption.
+        left; reflexivity.
+      }
+
+      remember (rootOf (fst (tree2Topo tr 0))) as oidx; clear Heqoidx.
+
+      (** Do case analysis per a rule. *)
+      apply in_app_or in H3; destruct H3.
+
+      1: { (** Rules per a child *)
+        apply concat_In in H1; destruct H1 as [crls [? ?]].
+        apply in_map_iff in H1; destruct H1 as [cidx [? ?]]; subst.
+
+        (** Derive that the child has the parent. *)
+        assert (parentIdxOf (fst (tree2Topo tr 0)) cidx = Some oidx)
+          by (apply subtreeChildrenIndsOf_parentIdxOf; auto).
+
+        dest_in.
+
+        { disc_rule_conds_ex; simpl_InvDirME_msgs; disc_InvDirME. }
+        
+        { (* [liGetSImmME] *)
+          disc_rule_conds_ex; disc_InvDirME.
+          { Ltac solve_InvDirME_by_silent :=
+              intros;
+              solve_MsgsP;
+              match goal with
+              | [H: _ -> NoRsI _ _ |- _] => apply H; auto
+              end;
+              fail.
+
+              solve_InvDirME_by_silent.
+          }
+          { intros.
+            red in H10; simpl in H10; dest; subst.
+            derive_child_idx_in oidx0.
+            assert (NoRsI oidx0 msgs)
+              by (solve_NoRsI_base; solve_NoRsI_by_rqUp oidx0).
+            solve_MsgsP.
+          }
+          { destruct (idx_dec cidx oidx0); subst.
+            { Ltac solve_InvDirME_by_idx_false :=
+                intros; subst topo; congruence.
+                
+                solve_InvDirME_by_idx_false.
+            }
+            { solve_InvDirME_by_silent. }
+          }
+        }
+
+        { disc_rule_conds_ex; simpl_InvDirME_msgs; disc_InvDirME. }
+
+        { (* [liGetMImm] *)
+          disc_rule_conds_ex; disc_InvDirME.
+          { solve_InvDirME_by_silent. }
+          { intros.
+            red in H10; simpl in H10; dest; subst.
+            derive_child_idx_in oidx0.
+            assert (NoRsI oidx0 msgs)
+              by (solve_NoRsI_base; solve_NoRsI_by_rqUp oidx0).
+            solve_MsgsP.
+          }
+          { destruct (idx_dec cidx oidx0); subst.
+            { solve_InvDirME_by_idx_false. }
+            { solve_InvDirME_by_silent. }
+          }
+        }
+
+        { disc_rule_conds_ex; simpl_InvDirME_msgs; disc_InvDirME. }
+        { disc_rule_conds_ex; simpl_InvDirME_msgs; disc_InvDirME. }
+
+        { (* [liInvImmI] *)
+          disc_rule_conds_ex; disc_InvDirME.
+          { solve_InvDirME_by_silent. }
+          { destruct (idx_dec cidx oidx0); subst.
+            { Ltac solve_InvDirME_by_dir_I :=
+                intros; exfalso;
+                eapply getDir_I_ObjDirMETo_false; eauto.
+
+                solve_InvDirME_by_dir_I.
+            }
+            { solve_InvDirME_by_silent. }
+          }
+          { destruct (idx_dec cidx oidx0); subst.
+            { solve_InvDirME_by_idx_false. }
+            { solve_InvDirME_by_silent. }
+          }
+        }
+
+        { disc_rule_conds_ex; disc_InvDirME.
+          { solve_InvDirME_by_silent. }
+          { Ltac solve_InvDirME_by_diff_dir :=
+              intros;
+              match goal with
+              | [Hn: ObjDirMETo _ _ |- _] =>
+                red in Hn; dest; simpl in *; solve_mesi
+              end.
+
+            solve_InvDirME_by_diff_dir.
+          }
+          { destruct (idx_dec cidx oidx0); subst.
+            { solve_InvDirME_by_idx_false. }
+            { solve_InvDirME_by_silent. }
+          }
+        }
+
+        { disc_rule_conds_ex; disc_InvDirME.
+          { solve_InvDirME_by_silent. }
+          { Ltac disc_getDir :=
+              try match goal with
+                  | [H: getDir _ _ = _ |- _] =>
+                    first [apply getDir_M_imp in H; destruct H
+                          |apply getDir_E_imp in H; destruct H
+                          |apply getDir_S_imp in H; destruct H]
+                  | [H: mesiE <= getDir _ _ |- _] =>
+                    apply getDir_ME_imp in H; destruct H
+                  end.
+
+            disc_getDir.
+            solve_InvDirME_by_diff_dir.
+          }
+          { destruct (idx_dec cidx oidx0); subst.
+            { solve_InvDirME_by_idx_false. }
+            { solve_InvDirME_by_silent. }
+          }
+        }
+
+        { disc_rule_conds_ex; disc_InvDirME.
+          { solve_InvDirME_by_silent. }
+          { solve_InvDirME_by_diff_dir. }
+          { destruct (idx_dec cidx oidx0); subst.
+            { solve_InvDirME_by_idx_false. }
+            { solve_InvDirME_by_silent. }
+          }
+        }
+
+        { disc_rule_conds_ex; disc_InvDirME.
+          { solve_InvDirME_by_silent. }
+          { destruct (idx_dec cidx oidx0); subst.
+            { solve_InvDirME_by_dir_I. }
+            { solve_InvDirME_by_silent. }
+          }
+          { destruct (idx_dec cidx oidx0); subst.
+            { solve_InvDirME_by_idx_false. }
+            { solve_InvDirME_by_silent. }
+          }
+        }
+
+        { disc_rule_conds_ex; disc_InvDirME.
+          { solve_InvDirME_by_silent. }
+          { disc_getDir.
+            solve_InvDirME_by_diff_dir.
+          }
+          { destruct (idx_dec cidx oidx0); subst.
+            { subst topo; disc_rule_conds_ex. }
+            { solve_InvDirME_by_silent. }
+          }
+        }
+
+        { disc_rule_conds_ex; disc_InvDirME.
+          { solve_InvDirME_by_silent. }
+          { solve_InvDirME_by_diff_dir. }
+          { destruct (idx_dec cidx oidx0); subst.
+            { solve_InvDirME_by_idx_false. }
+            { solve_InvDirME_by_silent. }
+          }
+        }
+
+      }
+
+      dest_in.
+
+      { disc_rule_conds_ex; simpl_InvDirME_msgs; disc_InvDirME.
+        solve_InvDirME_by_diff_dir.
+      }
+
+      { disc_rule_conds_ex.
+        disc_MesiDownLockInv oidx Hmdl.
+        simpl_InvDirME_msgs.
+        disc_InvDirME.
+
+        intros.
+        red in H20; simpl in H20; dest; subst.
+        derive_child_idx_in oidx0.
+
+        solve_NoRsI_base.
+
+        Ltac solve_NoRsI_by_parent_lock oidx :=
+          disc_MsgConflictsInv oidx;
+          match goal with
+          | [Hmcfp: ParentLockConflicts _ oidx _ _,
+                    Hin: InMPI _ (downTo oidx, ?msg) |- _] =>
+            specialize (Hmcfp ltac:(red; mred; simpl; eauto));
+            destruct Hmcfp as [Hmcfp _];
+            eapply (Hmcfp (downTo oidx, msg)); eauto
+          end.
+
+        solve_NoRsI_by_parent_lock oidx0.
+      }
+
+    - (*! Cases for Li caches *)
+
+      (** Derive some necessary information: each Li has a parent. *)
+      apply in_map_iff in H1; destruct H1 as [oidx [? ?]]; subst; simpl in *.
+
+      pose proof (tree2Topo_TreeTopoNode tr 0) as Htn.
+      pose proof (c_li_indices_tail_has_parent Htr _ _ H2).
+      destruct H1 as [pidx [? ?]].
+      pose proof (Htn _ _ H4); dest.
+
+      (** Do case analysis per a rule. *)
+      apply in_app_or in H3; destruct H3.
+
+      1: { (** Rules per a child *)
+        apply concat_In in H3; destruct H3 as [crls [? ?]].
+        apply in_map_iff in H3; destruct H3 as [cidx [? ?]]; subst.
+
+        (** Derive that the child has the parent. *)
+        assert (parentIdxOf (fst (tree2Topo tr 0)) cidx = Some oidx)
+          by (apply subtreeChildrenIndsOf_parentIdxOf; auto).
+
+        dest_in.
+
+        { disc_rule_conds_ex; simpl_InvDirME_msgs; disc_InvDirME. }
+
+        { disc_rule_conds_ex; disc_InvDirME.
+          { solve_InvDirME_by_silent. }
+          { intros.
+            red in H18; simpl in H18; dest; subst.
+            derive_child_idx_in oidx0.
+            assert (NoRsI oidx0 msgs)
+              by (solve_NoRsI_base; solve_NoRsI_by_rqUp oidx0).
+            solve_MsgsP.
+          }
+          { destruct (idx_dec cidx oidx0); subst.
+            { solve_InvDirME_by_idx_false. }
+            { solve_InvDirME_by_silent. }
+          }
+        }
+
+        { disc_rule_conds_ex; simpl_InvDirME_msgs; disc_InvDirME. }
+        { disc_rule_conds_ex; simpl_InvDirME_msgs; disc_InvDirME. }
+        { disc_rule_conds_ex; simpl_InvDirME_msgs; disc_InvDirME. }
+
+        { (* [liGetMImm] *)
+          disc_rule_conds_ex; disc_InvDirME.
+          { solve_InvDirME_by_silent. }
+          { intros.
+            red in H18; simpl in H18; dest; subst.
+            derive_child_idx_in oidx0.
+            assert (NoRsI oidx0 msgs)
+              by (solve_NoRsI_base; solve_NoRsI_by_rqUp oidx0).
+            solve_MsgsP.
+          }
+          { destruct (idx_dec cidx oidx0); subst.
+            { solve_InvDirME_by_idx_false. }
+            { solve_InvDirME_by_silent. }
+          }
+        }
+
+        { disc_rule_conds_ex; simpl_InvDirME_msgs; disc_InvDirME. }
+        { disc_rule_conds_ex; simpl_InvDirME_msgs; disc_InvDirME. }
+        { disc_rule_conds_ex; simpl_InvDirME_msgs; disc_InvDirME. }
+
+        { (* [liInvImmI] *)
+          disc_rule_conds_ex; disc_InvDirME.
+          { solve_InvDirME_by_silent. }
+          { destruct (idx_dec cidx oidx0); subst.
+            { solve_InvDirME_by_dir_I. }
+            { solve_InvDirME_by_silent. }
+          }
+          { destruct (idx_dec cidx oidx0); subst.
+            { solve_InvDirME_by_idx_false. }
+            { solve_InvDirME_by_silent. }
+          }
+        }
+
+        { disc_rule_conds_ex; disc_InvDirME.
+          { solve_InvDirME_by_silent. }
+          { solve_InvDirME_by_diff_dir. }
+          { destruct (idx_dec cidx oidx0); subst.
+            { solve_InvDirME_by_idx_false. }
+            { solve_InvDirME_by_silent. }
+          }
+        }
+
+        { disc_rule_conds_ex; disc_InvDirME.
+          { solve_InvDirME_by_silent. }
+          { disc_getDir.
+            solve_InvDirME_by_diff_dir.
+          }
+          { destruct (idx_dec cidx oidx0); subst.
+            { solve_InvDirME_by_idx_false. }
+            { solve_InvDirME_by_silent. }
+          }
+        }
+
+        { disc_rule_conds_ex; disc_InvDirME.
+          { solve_InvDirME_by_silent. }
+          { solve_InvDirME_by_diff_dir. }
+          { destruct (idx_dec cidx oidx0); subst.
+            { solve_InvDirME_by_idx_false. }
+            { solve_InvDirME_by_silent. }
+          }
+        }
+
+        { disc_rule_conds_ex; disc_InvDirME.
+          { solve_InvDirME_by_silent. }
+          { destruct (idx_dec cidx oidx0); subst.
+            { solve_InvDirME_by_dir_I. }
+            { solve_InvDirME_by_silent. }
+          }
+          { destruct (idx_dec cidx oidx0); subst.
+            { solve_InvDirME_by_idx_false. }
+            { solve_InvDirME_by_silent. }
+          }
+        }
+
+        { disc_rule_conds_ex; disc_InvDirME.
+          { solve_InvDirME_by_silent. }
+          { disc_getDir.
+            solve_InvDirME_by_diff_dir.
+          }
+          { destruct (idx_dec cidx oidx0); subst.
+            { subst topo; disc_rule_conds_ex. }
+            { solve_InvDirME_by_silent. }
+          }
+        }
+
+        { disc_rule_conds_ex; disc_InvDirME.
+          { solve_InvDirME_by_silent. }
+          { solve_InvDirME_by_diff_dir. }
+          { destruct (idx_dec cidx oidx0); subst.
+            { solve_InvDirME_by_idx_false. }
+            { solve_InvDirME_by_silent. }
+          }
+        }
+
+      }
+
+      dest_in.
+
+      { disc_rule_conds_ex; simpl_InvDirME_msgs; disc_InvDirME.
+        solve_InvDirME_by_diff_dir.
+      }
+
+      { disc_rule_conds_ex.
+        derive_footprint_info_basis oidx.
+        derive_child_chns cidx.
+        disc_rule_conds_ex.
+        simpl_InvDirME_msgs.
+        disc_InvDirME.
+
+        intros.
+        red in H29; simpl in H29; dest; subst.
+        derive_child_idx_in oidx0.
+        solve_NoRsI_base.
+        solve_NoRsI_by_parent_lock oidx0.
+      }
+
+      { disc_rule_conds_ex; simpl_InvDirME_msgs; disc_InvDirME.
+        solve_InvDirME_by_diff_dir.
+      }
+
+      { disc_rule_conds_ex; simpl_InvDirME_msgs; disc_InvDirME. }
+      { disc_rule_conds_ex; simpl_InvDirME_msgs; disc_InvDirME. }
+      { disc_rule_conds_ex; simpl_InvDirME_msgs; disc_InvDirME. }
+      { disc_rule_conds_ex; simpl_InvDirME_msgs; disc_InvDirME. }
+
+      { disc_rule_conds_ex; simpl_InvDirME_msgs; disc_InvDirME.
+        solve_InvDirME_by_diff_dir.
+      }
+
+      { disc_rule_conds_ex.
+        derive_footprint_info_basis oidx.
+        derive_child_chns cidx.
+        disc_rule_conds_ex.
+        simpl_InvDirME_msgs.
+        disc_InvDirME.
+
+        intros.
+        red in H29; simpl in H29; dest; subst.
+        derive_child_idx_in oidx0.
+        solve_NoRsI_base.
+        solve_NoRsI_by_parent_lock oidx0.
+      }
+
+      { disc_rule_conds_ex; simpl_InvDirME_msgs; disc_InvDirME. }
+
+      { disc_rule_conds_ex.
+        disc_MesiDownLockInv oidx Hmdl.
+        simpl_InvDirME_msgs.
+        disc_InvDirME.
+
+        intros.
+        red in H26; simpl in H26; dest; subst.
+        derive_child_idx_in oidx0.
+        solve_NoRsI_base.
+        solve_NoRsI_by_parent_lock oidx0.
+      }
+
+      { disc_rule_conds_ex; simpl_InvDirME_msgs; disc_InvDirME. }
+      { disc_rule_conds_ex; simpl_InvDirME_msgs; disc_InvDirME. }
+      { disc_rule_conds_ex; simpl_InvDirME_msgs; disc_InvDirME. }
+      { disc_rule_conds_ex; simpl_InvDirME_msgs; disc_InvDirME.
+        solve_InvDirME_by_diff_dir.
+      }
+
+      { disc_rule_conds_ex; simpl_InvDirME_msgs; disc_InvDirME. }
+      { disc_rule_conds_ex; simpl_InvDirME_msgs; disc_InvDirME. }
+      { disc_rule_conds_ex; simpl_InvDirME_msgs; disc_InvDirME. }
+      { disc_rule_conds_ex; simpl_InvDirME_msgs; disc_InvDirME. }
+      
+    - (*! Cases for L1 caches *)
+
+      (** Derive some necessary information: each Li has a parent. *)
+      apply in_map_iff in H1; destruct H1 as [oidx [? ?]]; subst.
+
+      pose proof (tree2Topo_TreeTopoNode tr 0) as Htn.
+      pose proof (c_l1_indices_has_parent Htr _ _ H2).
+      destruct H1 as [pidx [? ?]].
+      pose proof (Htn _ _ H4); dest.
+
+      (** Do case analysis per a rule. *)
+      dest_in.
+      all: disc_rule_conds_ex; simpl_InvDirME_msgs; disc_InvDirME.
+
+      (* END_SKIP_PROOF_OFF *)
+  Qed.
+
+End InvDirME.
+
 Definition InvWB (topo: DTree) (st: MState): Prop :=
   forall oidx pidx,
     parentIdxOf topo oidx = Some pidx ->
@@ -26,8 +700,9 @@ Definition InvWB (topo: DTree) (st: MState): Prop :=
       orq <+- (bst_orqs st)@[oidx];
       post <+- (bst_oss st)@[pidx];
       porq <+- (bst_orqs st)@[pidx];
-      (ObjDirME porq post oidx -> ObjInvWRq oidx (bst_msgs st) ->
-       ObjOwned ost).
+      (ObjDirME porq post oidx ->
+       (ost#[dir].(dir_st) <= mesiS \/ ObjInvWRq oidx (bst_msgs st)) ->
+       mesiS <= ost#[status]).
 
 Section InvWB.
   Variable (tr: tree).
@@ -45,9 +720,19 @@ Section InvWB.
     destruct (implORqsInit tr)@[oidx] as [orq|] eqn:Horq; simpl; auto.
     destruct (implOStatesInit tr)@[pidx] as [post|] eqn:Hpost; simpl; auto.
     destruct (implORqsInit tr)@[pidx] as [porq|] eqn:Hporq; simpl; auto.
-    intros.
-    do 2 (red in H1); dest.
-    do 2 (red in H1); dest_in.
+    intros; exfalso.
+    red in H0; dest.
+    destruct (in_dec idx_dec pidx (c_li_indices cifc ++ c_l1_indices cifc)).
+    - subst cifc; rewrite c_li_indices_head_rootOf in i by assumption.
+      inv i.
+      + rewrite implOStatesInit_value_root in Hpost by assumption.
+        inv Hpost.
+        simpl in *; solve_mesi.
+      + rewrite implOStatesInit_value_non_root in Hpost by assumption.
+        inv Hpost.
+        simpl in *; solve_mesi.
+    - rewrite implOStatesInit_None in Hpost by assumption.
+      discriminate.
   Qed.
 
   Lemma mesi_InvWB_ext_in:
@@ -64,12 +749,13 @@ Section InvWB.
     destruct (orqs@[oidx]) as [orq|] eqn:Horq; simpl in *; auto.
     destruct (oss@[pidx]) as [post|] eqn:Hpost; simpl in *; auto.
     destruct (orqs@[pidx]) as [porq|] eqn:Hporq; simpl in *; auto.
-    intros.
-    destruct H4 as [idm [? ?]].
-    apply InMP_enqMsgs_or in H4.
-    destruct H4; [|apply H; auto; do 2 red; eauto].
-    apply in_map with (f:= idOf) in H4; simpl in H4.
-    apply H1 in H4; simpl in H4.
+    intros; specialize (H H3); dest.
+    split; [assumption|intros].
+    destruct H5 as [idm [? ?]].
+    apply InMP_enqMsgs_or in H5.
+    destruct H5; [|apply H4; auto; do 2 red; eauto].
+    apply in_map with (f:= idOf) in H5; simpl in H5.
+    apply H1 in H5; simpl in H5.
     exfalso; eapply DisjList_In_1.
     - apply tree2Topo_minds_merqs_disj.
     - eassumption.
@@ -77,7 +763,7 @@ Section InvWB.
       + specialize (H0 oidx); simpl in H0.
         rewrite Host in H0; simpl in H0.
         eassumption.
-      + destruct idm as [midx msg]; inv H5.
+      + destruct idm as [midx msg]; inv H6.
         simpl; tauto.
   Qed.
 
@@ -96,10 +782,11 @@ Section InvWB.
     destruct (orqs@[oidx]) as [orq|] eqn:Horq; simpl in *; auto.
     destruct (oss@[pidx]) as [post|] eqn:Hpost; simpl in *; auto.
     destruct (orqs@[pidx]) as [porq|] eqn:Hporq; simpl in *; auto.
-    intros.
-    destruct H3 as [idm [? ?]].
-    apply InMP_deqMsgs in H3.
-    apply H; auto.
+    intros; specialize (H H2); dest.
+    split; [assumption|intros].
+    destruct H4 as [idm [? ?]].
+    apply InMP_deqMsgs in H4.
+    apply H3; auto.
     do 2 red; eauto.
   Qed.
 
@@ -117,12 +804,13 @@ Section InvWB.
     destruct (orqs@[oidx]) as [orq|] eqn:Horq; simpl in *; auto.
     destruct (oss@[pidx]) as [post|] eqn:Hpost; simpl in *; auto.
     destruct (orqs@[pidx]) as [porq|] eqn:Hporq; simpl in *; auto.
-    intros.
-    apply H; auto.
-    destruct H3 as [idm [? ?]].
-    apply InMP_enqMP_or in H3; destruct H3.
+    intros; specialize (H H2); dest.
+    split; [assumption|intros].
+    apply H3; auto.
+    destruct H4 as [idm [? ?]].
+    apply InMP_enqMP_or in H4; destruct H4.
     - dest; subst.
-      exfalso; inv H4; auto.
+      exfalso; inv H5; auto.
     - do 2 red; eauto.
   Qed.
   
@@ -155,11 +843,11 @@ Section InvWB.
     destruct (orqs@[oidx]) as [orq|] eqn:Horq; simpl in *; auto.
     destruct (oss@[pidx]) as [post|] eqn:Hpost; simpl in *; auto.
     destruct (orqs@[pidx]) as [porq|] eqn:Hporq; simpl in *; auto.
-    intros.
-    apply H; auto.
-    destruct H2 as [idm [? ?]].
-    apply InMP_deqMP in H2.
-    do 2 red; eauto.
+    intros; specialize (H H1); dest.
+    split; [assumption|intros].
+    destruct H3 as [idm [? ?]].
+    apply InMP_deqMP in H3.
+    apply H2; do 2 red; eauto.
   Qed.
 
   Lemma InvWB_deqMsgs:
@@ -175,11 +863,11 @@ Section InvWB.
     destruct (orqs@[oidx]) as [orq|] eqn:Horq; simpl in *; auto.
     destruct (oss@[pidx]) as [post|] eqn:Hpost; simpl in *; auto.
     destruct (orqs@[pidx]) as [porq|] eqn:Hporq; simpl in *; auto.
-    intros.
-    apply H; auto.
-    destruct H2 as [idm [? ?]].
-    apply InMP_deqMsgs in H2.
-    do 2 red; eauto.
+    intros; specialize (H H1); dest.
+    split; [assumption|intros].
+    destruct H3 as [idm [? ?]].
+    apply InMP_deqMsgs in H3.
+    apply H2; do 2 red; eauto.
   Qed.
 
   Ltac simpl_InvWB_msgs_enqMP :=
@@ -208,9 +896,12 @@ Section InvWB.
     repeat
       match goal with
       | |- _ <+- ?ov; _ =>
-        let Hv := fresh "H" in
-        let v := fresh "v" in
-        destruct ov as [v|] eqn:Hv; simpl in *; [|auto]
+        first [match goal with
+               | [H: ov = _ |- _] => rewrite H in *; simpl in *
+               end
+              |let Hov := fresh "H" in
+               let v := fresh "v" in
+               destruct ov as [v|] eqn:Hov; simpl in *; [|auto]]
       end.
 
   Ltac disc_InvWB :=
@@ -313,72 +1004,122 @@ Section InvWB.
         { disc_rule_conds_ex.
           simpl_InvWB_msgs.
           disc_InvWB.
+          mred.
         }
 
         { disc_rule_conds_ex.
           derive_child_idx_in cidx.
           simpl_InvWB_msgs.
           disc_InvWB.
-          { assert (NoRqI oidx msgs)
-              by (solve_NoRqI_base; solve_NoRqI_by_no_locks oidx).
-            solve_InvWB_by_NoRqI.
+          { intros; split.
+            { intros; red; simpl.
+              destruct (fst (snd os)); intuition solve_mesi.
+            }
+            { assert (NoRqI oidx msgs)
+                by (solve_NoRqI_base; solve_NoRqI_by_no_locks oidx).
+              solve_InvWB_by_NoRqI.
+            }
           }
           { intros.
             red in H17; simpl in H17; dest; subst.
-            assert (NoRqI oidx0 msgs)
-              by (solve_NoRqI_base; solve_NoRqI_by_rqUp oidx0).
-            solve_InvWB_by_NoRqI.
+            split.
+            {
+
+              Ltac derive_uplock_by_rqUp cidx :=
+                disc_MsgConflictsInv cidx;
+                (* TODO: must be in [disc_MsgConflictsInv]? *)
+                match goal with
+                | [Hcf: forall _ _, parentIdxOf _ cidx = Some _ -> _,
+                     Hp: parentIdxOf _ cidx = Some ?pidx,
+                     Ho: _@[?pidx] = Some _ |- _] =>
+                  specialize (Hcf _ _ Hp Ho); destruct Hcf
+                end;
+                match goal with
+                | [H: RqUpConflicts cidx _ _,
+                      Hr: FirstMPI _ (rqUpFrom cidx, ?rmsg) |- _] =>
+                  specialize (H (rqUpFrom cidx, rmsg) eq_refl (FirstMP_InMP Hr)); dest
+                end.
+
+                derive_uplock_by_rqUp oidx0.
+
+                destruct (v0@[upRq]); [intros; discriminate|exfalso; auto].
+            }
+            { assert (NoRqI oidx0 msgs)
+                by (solve_NoRqI_base; solve_NoRqI_by_rqUp oidx0).
+              solve_InvWB_by_NoRqI.
+            }
           }
         }
 
         { disc_rule_conds_ex.
           simpl_InvWB_msgs.
           disc_InvWB.
-          solve_InvWB_by_downlock.
+          { mred. }
+          { solve_InvWB_by_downlock. }
         }
 
         { disc_rule_conds_ex.
           derive_child_idx_in cidx.
           simpl_InvWB_msgs.
           disc_InvWB.
-          { assert (NoRqI oidx msgs)
-              by (solve_NoRqI_base; solve_NoRqI_by_no_locks oidx).
-            solve_InvWB_by_NoRqI.
+          { intros; split.
+            { intros; red; simpl.
+              destruct (fst (snd os)); intuition solve_mesi.
+            }
+            { assert (NoRqI oidx msgs)
+                by (solve_NoRqI_base; solve_NoRqI_by_no_locks oidx).
+              solve_InvWB_by_NoRqI.
+            }
           }
           { intros.
             red in H17; simpl in H17; dest; subst.
-            assert (NoRqI oidx0 msgs)
-              by (solve_NoRqI_base; solve_NoRqI_by_rqUp oidx0).
-            solve_InvWB_by_NoRqI.
+            split.
+            { derive_uplock_by_rqUp oidx0.
+              destruct (v0@[upRq]); [intros; discriminate|exfalso; auto].
+            }
+            { assert (NoRqI oidx0 msgs)
+                by (solve_NoRqI_base; solve_NoRqI_by_rqUp oidx0).
+              solve_InvWB_by_NoRqI.
+            }
           }
         }
 
         { disc_rule_conds_ex.
           simpl_InvWB_msgs.
           disc_InvWB.
-          solve_InvWB_by_downlock.
+          { mred. }
+          { solve_InvWB_by_downlock. }
         }
 
         { disc_rule_conds_ex.
           simpl_InvWB_msgs.
           disc_InvWB.
-          solve_InvWB_by_downlock.
+          { mred. }
+          { solve_InvWB_by_downlock. }
         }
 
         { disc_rule_conds_ex.
           simpl_InvWB_msgs.
           disc_InvWB.
+          mred.
         }
 
         { disc_rule_conds_ex.
           simpl_InvWB_msgs.
           disc_InvWB.
-          solve_InvWB_by_diff_dir.
+          { intros; split.
+            { intros.
+              admit.
+            }
+            { intros; apply H0; auto. }
+          }
+          { solve_InvWB_by_diff_dir. }
         }
 
         { disc_rule_conds_ex.
           simpl_InvWB_msgs.
           disc_InvWB.
+          mred.
         }
 
         { disc_rule_conds_ex.
